Initial F* extraction of `flaand`

proofs/fstar/extraction/Polytune.Faand.fst
@@ -6,7 +6,9 @@ open FStar.Mul
 let _ =
   (* This module has implicit dependencies, here we make them explicit. *)
   (* The implicit dependencies arise from typeclasses instances. *)
+  let open Blake3 in
   let open Polytune.Channel in
+  let open Polytune.Data_types in
   let open Rand.Distributions.Distribution in
   let open Rand.Distributions.Other in
   let open Serde.De in
@@ -43,6 +45,135 @@ let impl: Core.Convert.t_From t_Error Polytune.Channel.t_Error =
     f_from_post = (fun (e: Polytune.Channel.t_Error) (out: t_Error) -> true);
     f_from = fun (e: Polytune.Channel.t_Error) -> Error_ChannelErr e <: t_Error
   }
+
+/// Represents a cryptographic commitment as a fixed-size 32-byte array (a BLAKE3 hash).
+type t_Commitment = | Commitment : t_Array u8 (mk_usize 32) -> t_Commitment
+
+[@@ FStar.Tactics.Typeclasses.tcinstance]
+assume
+val impl_2': Core.Fmt.t_Debug t_Commitment
+
+let impl_2 = impl_2'
+
+[@@ FStar.Tactics.Typeclasses.tcinstance]
+assume
+val impl_3': Core.Clone.t_Clone t_Commitment
+
+let impl_3 = impl_3'
+
+[@@ FStar.Tactics.Typeclasses.tcinstance]
+assume
+val e___impl': Serde.Ser.t_Serialize t_Commitment
+
+let e___impl = e___impl'
+
+[@@ FStar.Tactics.Typeclasses.tcinstance]
+assume
+val e_ee_1__impl': Serde.De.t_Deserialize t_Commitment
+
+let e_ee_1__impl = e_ee_1__impl'
+
+[@@ FStar.Tactics.Typeclasses.tcinstance]
+assume
+val impl_6': Core.Cmp.t_PartialEq t_Commitment t_Commitment
+
+let impl_6 = impl_6'
+
+/// Commits to a value using the BLAKE3 cryptographic hash function.
+/// This is not a general-purpose commitment scheme, the input value is assumed to have high entropy.
+let commit (value: t_Slice u8) : t_Commitment =
+  Commitment
+  (Core.Convert.f_into #Blake3.t_Hash
+      #(t_Array u8 (mk_usize 32))
+      #FStar.Tactics.Typeclasses.solve
+      (Blake3.hash value <: Blake3.t_Hash))
+  <:
+  t_Commitment
+
+/// Verifies if a given value matches a previously generated commitment.
+/// This is not a general-purpose commitment scheme, the input value is assumed to have high entropy.
+let open_commitment (commitment: t_Commitment) (value: t_Slice u8) : bool =
+  (Blake3.impl_Hash__as_bytes (Blake3.hash value <: Blake3.t_Hash) <: t_Array u8 (mk_usize 32)) =.
+  commitment._0
+
+/// Implements broadcast with abort based on Goldwasser and Lindell\'s protocol
+/// for all parties at once, where each party sends its vector to all others.
+/// The function returns the vector received and verified by broadcast.
+assume
+val broadcast':
+    #v_T: Type0 ->
+    #iimpl_951670863_: Type0 ->
+    {| i2: Core.Clone.t_Clone v_T |} ->
+    {| i3: Serde.Ser.t_Serialize v_T |} ->
+    {| i4: Serde.De.t_DeserializeOwned v_T |} ->
+    {| i5: Core.Fmt.t_Debug v_T |} ->
+    {| i6: Core.Cmp.t_PartialEq v_T v_T |} ->
+    {| i7: Polytune.Channel.t_Channel iimpl_951670863_ |} ->
+    channel: iimpl_951670863_ ->
+    i: usize ->
+    n: usize ->
+    phase: string ->
+    vec: t_Slice v_T ->
+    len: usize
+  -> (iimpl_951670863_ &
+      Core.Result.t_Result
+        (Alloc.Vec.t_Vec (Alloc.Vec.t_Vec v_T Alloc.Alloc.t_Global) Alloc.Alloc.t_Global) t_Error)
+
+let broadcast
+      (#v_T #iimpl_951670863_: Type0)
+      (#[FStar.Tactics.Typeclasses.tcresolve ()] i2: Core.Clone.t_Clone v_T)
+      (#[FStar.Tactics.Typeclasses.tcresolve ()] i3: Serde.Ser.t_Serialize v_T)
+      (#[FStar.Tactics.Typeclasses.tcresolve ()] i4: Serde.De.t_DeserializeOwned v_T)
+      (#[FStar.Tactics.Typeclasses.tcresolve ()] i5: Core.Fmt.t_Debug v_T)
+      (#[FStar.Tactics.Typeclasses.tcresolve ()] i6: Core.Cmp.t_PartialEq v_T v_T)
+      (#[FStar.Tactics.Typeclasses.tcresolve ()] i7: Polytune.Channel.t_Channel iimpl_951670863_)
+     = broadcast' #v_T #iimpl_951670863_ #i2 #i3 #i4 #i5 #i6 #i7
+
+/// Implements same broadcast with abort as broadcast, but only the first element of the tuple in
+/// the vector is broadcasted, the second element is simply sent to all parties.
+assume
+val broadcast_first_send_second':
+    #v_T: Type0 ->
+    #v_S: Type0 ->
+    #iimpl_951670863_: Type0 ->
+    {| i3: Core.Clone.t_Clone v_T |} ->
+    {| i4: Serde.Ser.t_Serialize v_T |} ->
+    {| i5: Serde.De.t_DeserializeOwned v_T |} ->
+    {| i6: Core.Fmt.t_Debug v_T |} ->
+    {| i7: Core.Cmp.t_PartialEq v_T v_T |} ->
+    {| i8: Core.Clone.t_Clone v_S |} ->
+    {| i9: Serde.Ser.t_Serialize v_S |} ->
+    {| i10: Serde.De.t_DeserializeOwned v_S |} ->
+    {| i11: Core.Fmt.t_Debug v_S |} ->
+    {| i12: Core.Cmp.t_PartialEq v_S v_S |} ->
+    {| i13: Polytune.Channel.t_Channel iimpl_951670863_ |} ->
+    channel: iimpl_951670863_ ->
+    i: usize ->
+    n: usize ->
+    phase: string ->
+    vec: t_Slice (Alloc.Vec.t_Vec (v_T & v_S) Alloc.Alloc.t_Global) ->
+    len: usize
+  -> (iimpl_951670863_ &
+      Core.Result.t_Result
+        (Alloc.Vec.t_Vec (Alloc.Vec.t_Vec (v_T & v_S) Alloc.Alloc.t_Global) Alloc.Alloc.t_Global)
+        t_Error)
+
+let broadcast_first_send_second
+      (#v_T #v_S #iimpl_951670863_: Type0)
+      (#[FStar.Tactics.Typeclasses.tcresolve ()] i3: Core.Clone.t_Clone v_T)
+      (#[FStar.Tactics.Typeclasses.tcresolve ()] i4: Serde.Ser.t_Serialize v_T)
+      (#[FStar.Tactics.Typeclasses.tcresolve ()] i5: Serde.De.t_DeserializeOwned v_T)
+      (#[FStar.Tactics.Typeclasses.tcresolve ()] i6: Core.Fmt.t_Debug v_T)
+      (#[FStar.Tactics.Typeclasses.tcresolve ()] i7: Core.Cmp.t_PartialEq v_T v_T)
+      (#[FStar.Tactics.Typeclasses.tcresolve ()] i8: Core.Clone.t_Clone v_S)
+      (#[FStar.Tactics.Typeclasses.tcresolve ()] i9: Serde.Ser.t_Serialize v_S)
+      (#[FStar.Tactics.Typeclasses.tcresolve ()] i10: Serde.De.t_DeserializeOwned v_S)
+      (#[FStar.Tactics.Typeclasses.tcresolve ()] i11: Core.Fmt.t_Debug v_S)
+      (#[FStar.Tactics.Typeclasses.tcresolve ()] i12: Core.Cmp.t_PartialEq v_S v_S)
+      (#[FStar.Tactics.Typeclasses.tcresolve ()] i13: Polytune.Channel.t_Channel iimpl_951670863_)
+     =
+  broadcast_first_send_second' #v_T #v_S #iimpl_951670863_ #i3 #i4 #i5 #i6 #i7 #i8 #i9 #i10 #i11
+    #i12 #i13
 
 /// Protocol Pi_HaAND that performs F_HaAND from the paper
 /// [Global-Scale Secure Multiparty Computation](https://dl.acm.org/doi/pdf/10.1145/3133956.3133979).
@@ -405,3 +536,1374 @@ let fhaand
         <:
         (iimpl_951670863_ & Core.Result.t_Result (Alloc.Vec.t_Vec bool Alloc.Alloc.t_Global) t_Error
         )
+
+/// This function takes a 128-bit unsigned integer (`u128`) as input and produces a 128-bit hash value.
+/// We use the BLAKE3 cryptographic hash function to hash the input value and return the resulting hash.
+/// The hash is truncated to 128 bits to match the input size. Due to the truncation, the security
+/// guarantees of the hash function are reduced to 64-bit collision resistance and 128-bit preimage
+/// resistance. This is sufficient for the purposes of the protocol if RHO <= 64, which we expect
+/// to be the case in all real-world usages of our protocol.
+assume
+val hash128': input: u128 -> Core.Result.t_Result u128 t_Error
+
+let hash128 = hash128'
+
+/// Protocol Pi_LaAND that performs F_LaAND from the paper
+/// [Global-Scale Secure Multiparty Computation](https://dl.acm.org/doi/pdf/10.1145/3133956.3133979).
+/// This asynchronous function implements the \"leaky authenticated AND\" protocol. It computes
+/// shares <x>, <y>, and <z> such that the AND of the XORs of the input values x and y equals
+/// the XOR of the output values z.
+let flaand
+      (#iimpl_951670863_: Type0)
+      (#[FStar.Tactics.Typeclasses.tcresolve ()] i1: Polytune.Channel.t_Channel iimpl_951670863_)
+      (channel: iimpl_951670863_)
+      (delta: Polytune.Data_types.t_Delta)
+      (xshares, yshares, rshares:
+          (t_Slice Polytune.Data_types.t_Share & t_Slice Polytune.Data_types.t_Share &
+            t_Slice Polytune.Data_types.t_Share))
+      (i: usize)
+      (n: usize)
+      (l: usize)
+    : (iimpl_951670863_ &
+      Core.Result.t_Result (Alloc.Vec.t_Vec Polytune.Data_types.t_Share Alloc.Alloc.t_Global)
+        t_Error) =
+  if
+    (Core.Slice.impl__len #Polytune.Data_types.t_Share xshares <: usize) <>. l ||
+    (Core.Slice.impl__len #Polytune.Data_types.t_Share yshares <: usize) <>. l ||
+    (Core.Slice.impl__len #Polytune.Data_types.t_Share rshares <: usize) <>. l
+  then
+    channel,
+    (Core.Result.Result_Err (Error_InvalidLength <: t_Error)
+      <:
+      Core.Result.t_Result (Alloc.Vec.t_Vec Polytune.Data_types.t_Share Alloc.Alloc.t_Global)
+        t_Error)
+    <:
+    (iimpl_951670863_ &
+      Core.Result.t_Result (Alloc.Vec.t_Vec Polytune.Data_types.t_Share Alloc.Alloc.t_Global)
+        t_Error)
+  else
+    let y:Alloc.Vec.t_Vec bool Alloc.Alloc.t_Global =
+      Core.Iter.Traits.Iterator.f_collect #(Core.Iter.Adapters.Map.t_Map
+            (Core.Iter.Adapters.Take.t_Take (Core.Slice.Iter.t_Iter Polytune.Data_types.t_Share))
+            (Polytune.Data_types.t_Share -> bool))
+        #FStar.Tactics.Typeclasses.solve
+        #(Alloc.Vec.t_Vec bool Alloc.Alloc.t_Global)
+        (Core.Iter.Traits.Iterator.f_map #(Core.Iter.Adapters.Take.t_Take
+              (Core.Slice.Iter.t_Iter Polytune.Data_types.t_Share))
+            #FStar.Tactics.Typeclasses.solve
+            #bool
+            (Core.Iter.Traits.Iterator.f_take #(Core.Slice.Iter.t_Iter Polytune.Data_types.t_Share)
+                #FStar.Tactics.Typeclasses.solve
+                (Core.Slice.impl__iter #Polytune.Data_types.t_Share yshares
+                  <:
+                  Core.Slice.Iter.t_Iter Polytune.Data_types.t_Share)
+                l
+              <:
+              Core.Iter.Adapters.Take.t_Take (Core.Slice.Iter.t_Iter Polytune.Data_types.t_Share))
+            (fun share ->
+                let share:Polytune.Data_types.t_Share = share in
+                share.Polytune.Data_types._0)
+          <:
+          Core.Iter.Adapters.Map.t_Map
+            (Core.Iter.Adapters.Take.t_Take (Core.Slice.Iter.t_Iter Polytune.Data_types.t_Share))
+            (Polytune.Data_types.t_Share -> bool))
+    in
+    let tmp0, out:(iimpl_951670863_ &
+      Core.Result.t_Result (Alloc.Vec.t_Vec bool Alloc.Alloc.t_Global) t_Error) =
+      fhaand #iimpl_951670863_ channel delta i n l xshares y
+    in
+    let channel:iimpl_951670863_ = tmp0 in
+    match out <: Core.Result.t_Result (Alloc.Vec.t_Vec bool Alloc.Alloc.t_Global) t_Error with
+    | Core.Result.Result_Ok v ->
+      let z:Alloc.Vec.t_Vec bool Alloc.Alloc.t_Global = Alloc.Vec.from_elem #bool false l in
+      let e:Alloc.Vec.t_Vec bool Alloc.Alloc.t_Global = Alloc.Vec.from_elem #bool false l in
+      let zshares:Alloc.Vec.t_Vec Polytune.Data_types.t_Share Alloc.Alloc.t_Global =
+        Alloc.Vec.from_elem #Polytune.Data_types.t_Share
+          (Polytune.Data_types.Share false
+              (Polytune.Data_types.Auth
+                (Smallvec.impl_17__from_elem #(t_Array
+                        (Polytune.Data_types.t_Mac & Polytune.Data_types.t_Key) (mk_usize 2))
+                    ((Polytune.Data_types.Mac (mk_u128 0) <: Polytune.Data_types.t_Mac),
+                      (Polytune.Data_types.Key (mk_u128 0) <: Polytune.Data_types.t_Key)
+                      <:
+                      (Polytune.Data_types.t_Mac & Polytune.Data_types.t_Key))
+                    n
+                  <:
+                  Smallvec.t_SmallVec
+                  (t_Array (Polytune.Data_types.t_Mac & Polytune.Data_types.t_Key) (mk_usize 2)))
+                <:
+                Polytune.Data_types.t_Auth)
+            <:
+            Polytune.Data_types.t_Share)
+          l
+      in
+      let e, z, zshares:(Alloc.Vec.t_Vec bool Alloc.Alloc.t_Global &
+        Alloc.Vec.t_Vec bool Alloc.Alloc.t_Global &
+        Alloc.Vec.t_Vec Polytune.Data_types.t_Share Alloc.Alloc.t_Global) =
+        Rust_primitives.Hax.Folds.fold_range (mk_usize 0)
+          l
+          (fun temp_0_ temp_1_ ->
+              let e, z, zshares:(Alloc.Vec.t_Vec bool Alloc.Alloc.t_Global &
+                Alloc.Vec.t_Vec bool Alloc.Alloc.t_Global &
+                Alloc.Vec.t_Vec Polytune.Data_types.t_Share Alloc.Alloc.t_Global) =
+                temp_0_
+              in
+              let _:usize = temp_1_ in
+              true)
+          (e, z, zshares
+            <:
+            (Alloc.Vec.t_Vec bool Alloc.Alloc.t_Global & Alloc.Vec.t_Vec bool Alloc.Alloc.t_Global &
+              Alloc.Vec.t_Vec Polytune.Data_types.t_Share Alloc.Alloc.t_Global))
+          (fun temp_0_ ll ->
+              let e, z, zshares:(Alloc.Vec.t_Vec bool Alloc.Alloc.t_Global &
+                Alloc.Vec.t_Vec bool Alloc.Alloc.t_Global &
+                Alloc.Vec.t_Vec Polytune.Data_types.t_Share Alloc.Alloc.t_Global) =
+                temp_0_
+              in
+              let ll:usize = ll in
+              let z:Alloc.Vec.t_Vec bool Alloc.Alloc.t_Global =
+                Rust_primitives.Hax.Monomorphized_update_at.update_at_usize z
+                  ll
+                  (Core.Ops.Bit.f_bitxor (v.[ ll ] <: bool)
+                      (Core.Ops.Bit.f_bitand (xshares.[ ll ] <: Polytune.Data_types.t_Share)
+                            .Polytune.Data_types._0
+                          (yshares.[ ll ] <: Polytune.Data_types.t_Share).Polytune.Data_types._0
+                        <:
+                        bool)
+                    <:
+                    bool)
+              in
+              let e:Alloc.Vec.t_Vec bool Alloc.Alloc.t_Global =
+                Rust_primitives.Hax.Monomorphized_update_at.update_at_usize e
+                  ll
+                  (Core.Ops.Bit.f_bitxor (z.[ ll ] <: bool)
+                      (rshares.[ ll ] <: Polytune.Data_types.t_Share).Polytune.Data_types._0
+                    <:
+                    bool)
+              in
+              let zshares:Alloc.Vec.t_Vec Polytune.Data_types.t_Share Alloc.Alloc.t_Global =
+                Rust_primitives.Hax.Monomorphized_update_at.update_at_usize zshares
+                  ll
+                  ({
+                      (zshares.[ ll ] <: Polytune.Data_types.t_Share) with
+                      Polytune.Data_types._0 = z.[ ll ] <: bool
+                    }
+                    <:
+                    Polytune.Data_types.t_Share)
+              in
+              e, z, zshares
+              <:
+              (Alloc.Vec.t_Vec bool Alloc.Alloc.t_Global & Alloc.Vec.t_Vec bool Alloc.Alloc.t_Global &
+                Alloc.Vec.t_Vec Polytune.Data_types.t_Share Alloc.Alloc.t_Global))
+      in
+      let _:Prims.unit = Core.Mem.drop #(Alloc.Vec.t_Vec bool Alloc.Alloc.t_Global) v in
+      let _:Prims.unit = Core.Mem.drop #(Alloc.Vec.t_Vec bool Alloc.Alloc.t_Global) z in
+      let phi:Alloc.Vec.t_Vec u128 Alloc.Alloc.t_Global = Alloc.Vec.from_elem #u128 (mk_u128 0) l in
+      let phi:Alloc.Vec.t_Vec u128 Alloc.Alloc.t_Global =
+        Rust_primitives.Hax.Folds.fold_range (mk_usize 0)
+          l
+          (fun phi temp_1_ ->
+              let phi:Alloc.Vec.t_Vec u128 Alloc.Alloc.t_Global = phi in
+              let _:usize = temp_1_ in
+              true)
+          phi
+          (fun phi ll ->
+              let phi:Alloc.Vec.t_Vec u128 Alloc.Alloc.t_Global = phi in
+              let ll:usize = ll in
+              let phi:Alloc.Vec.t_Vec u128 Alloc.Alloc.t_Global =
+                Core.Iter.Traits.Iterator.f_fold (Core.Iter.Traits.Collect.f_into_iter #(Core.Iter.Adapters.Filter.t_Filter
+                          (Core.Ops.Range.t_Range usize) (usize -> bool))
+                      #FStar.Tactics.Typeclasses.solve
+                      (Core.Iter.Traits.Iterator.f_filter #(Core.Ops.Range.t_Range usize)
+                          #FStar.Tactics.Typeclasses.solve
+                          ({ Core.Ops.Range.f_start = mk_usize 0; Core.Ops.Range.f_end = n }
+                            <:
+                            Core.Ops.Range.t_Range usize)
+                          (fun k ->
+                              let k:usize = k in
+                              k <>. i <: bool)
+                        <:
+                        Core.Iter.Adapters.Filter.t_Filter (Core.Ops.Range.t_Range usize)
+                          (usize -> bool))
+                    <:
+                    Core.Iter.Adapters.Filter.t_Filter (Core.Ops.Range.t_Range usize)
+                      (usize -> bool))
+                  phi
+                  (fun phi k ->
+                      let phi:Alloc.Vec.t_Vec u128 Alloc.Alloc.t_Global = phi in
+                      let k:usize = k in
+                      let mk_yi, ki_yk:(Polytune.Data_types.t_Mac & Polytune.Data_types.t_Key) =
+                        (yshares.[ ll ] <: Polytune.Data_types.t_Share).Polytune.Data_types._1
+                          .Polytune.Data_types._0.[ k ]
+                      in
+                      let phi:Alloc.Vec.t_Vec u128 Alloc.Alloc.t_Global =
+                        Rust_primitives.Hax.Monomorphized_update_at.update_at_usize phi
+                          ll
+                          (((phi.[ ll ] <: u128) ^. ki_yk.Polytune.Data_types._0 <: u128) ^.
+                            mk_yi.Polytune.Data_types._0
+                            <:
+                            u128)
+                      in
+                      phi)
+              in
+              let phi:Alloc.Vec.t_Vec u128 Alloc.Alloc.t_Global =
+                Rust_primitives.Hax.Monomorphized_update_at.update_at_usize phi
+                  ll
+                  ((phi.[ ll ] <: u128) ^.
+                    ((cast ((yshares.[ ll ] <: Polytune.Data_types.t_Share).Polytune.Data_types._0
+                            <:
+                            bool)
+                        <:
+                        u128) *!
+                      delta.Polytune.Data_types._0
+                      <:
+                      u128)
+                    <:
+                    u128)
+              in
+              phi)
+      in
+      let ki_xj_phi:Alloc.Vec.t_Vec (Alloc.Vec.t_Vec u128 Alloc.Alloc.t_Global) Alloc.Alloc.t_Global
+      =
+        Alloc.Vec.from_elem #(Alloc.Vec.t_Vec u128 Alloc.Alloc.t_Global)
+          (Alloc.Vec.from_elem #u128 (mk_u128 0) l <: Alloc.Vec.t_Vec u128 Alloc.Alloc.t_Global)
+          n
+      in
+      let ei_uij:Alloc.Vec.t_Vec (Alloc.Vec.t_Vec (bool & u128) Alloc.Alloc.t_Global)
+        Alloc.Alloc.t_Global =
+        Alloc.Vec.from_elem #(Alloc.Vec.t_Vec (bool & u128) Alloc.Alloc.t_Global)
+          (Alloc.Vec.impl__new #(bool & u128) ()
+            <:
+            Alloc.Vec.t_Vec (bool & u128) Alloc.Alloc.t_Global)
+          n
+      in
+      (match
+          Rust_primitives.Hax.Folds.fold_return (Core.Iter.Traits.Collect.f_into_iter #(Core.Iter.Adapters.Filter.t_Filter
+                    (Core.Ops.Range.t_Range usize) (usize -> bool))
+                #FStar.Tactics.Typeclasses.solve
+                (Core.Iter.Traits.Iterator.f_filter #(Core.Ops.Range.t_Range usize)
+                    #FStar.Tactics.Typeclasses.solve
+                    ({ Core.Ops.Range.f_start = mk_usize 0; Core.Ops.Range.f_end = n }
+                      <:
+                      Core.Ops.Range.t_Range usize)
+                    (fun j ->
+                        let j:usize = j in
+                        j <>. i <: bool)
+                  <:
+                  Core.Iter.Adapters.Filter.t_Filter (Core.Ops.Range.t_Range usize) (usize -> bool))
+              <:
+              Core.Iter.Adapters.Filter.t_Filter (Core.Ops.Range.t_Range usize) (usize -> bool))
+            (ei_uij, ki_xj_phi
+              <:
+              (Alloc.Vec.t_Vec (Alloc.Vec.t_Vec (bool & u128) Alloc.Alloc.t_Global)
+                  Alloc.Alloc.t_Global &
+                Alloc.Vec.t_Vec (Alloc.Vec.t_Vec u128 Alloc.Alloc.t_Global) Alloc.Alloc.t_Global))
+            (fun temp_0_ j ->
+                let ei_uij, ki_xj_phi:(Alloc.Vec.t_Vec
+                    (Alloc.Vec.t_Vec (bool & u128) Alloc.Alloc.t_Global) Alloc.Alloc.t_Global &
+                  Alloc.Vec.t_Vec (Alloc.Vec.t_Vec u128 Alloc.Alloc.t_Global) Alloc.Alloc.t_Global)
+                =
+                  temp_0_
+                in
+                let j:usize = j in
+                match
+                  Rust_primitives.Hax.Folds.fold_return (Core.Iter.Traits.Collect.f_into_iter #(Core.Iter.Adapters.Take.t_Take
+                          (Core.Iter.Adapters.Enumerate.t_Enumerate (Core.Slice.Iter.t_Iter u128)))
+                        #FStar.Tactics.Typeclasses.solve
+                        (Core.Iter.Traits.Iterator.f_take #(Core.Iter.Adapters.Enumerate.t_Enumerate
+                              (Core.Slice.Iter.t_Iter u128))
+                            #FStar.Tactics.Typeclasses.solve
+                            (Core.Iter.Traits.Iterator.f_enumerate #(Core.Slice.Iter.t_Iter u128)
+                                #FStar.Tactics.Typeclasses.solve
+                                (Core.Slice.impl__iter #u128
+                                    (Core.Ops.Deref.f_deref #(Alloc.Vec.t_Vec u128
+                                            Alloc.Alloc.t_Global)
+                                        #FStar.Tactics.Typeclasses.solve
+                                        phi
+                                      <:
+                                      t_Slice u128)
+                                  <:
+                                  Core.Slice.Iter.t_Iter u128)
+                              <:
+                              Core.Iter.Adapters.Enumerate.t_Enumerate (Core.Slice.Iter.t_Iter u128)
+                            )
+                            l
+                          <:
+                          Core.Iter.Adapters.Take.t_Take
+                          (Core.Iter.Adapters.Enumerate.t_Enumerate (Core.Slice.Iter.t_Iter u128)))
+                      <:
+                      Core.Iter.Adapters.Take.t_Take
+                      (Core.Iter.Adapters.Enumerate.t_Enumerate (Core.Slice.Iter.t_Iter u128)))
+                    (ei_uij, ki_xj_phi
+                      <:
+                      (Alloc.Vec.t_Vec (Alloc.Vec.t_Vec (bool & u128) Alloc.Alloc.t_Global)
+                          Alloc.Alloc.t_Global &
+                        Alloc.Vec.t_Vec (Alloc.Vec.t_Vec u128 Alloc.Alloc.t_Global)
+                          Alloc.Alloc.t_Global))
+                    (fun temp_0_ temp_1_ ->
+                        let ei_uij, ki_xj_phi:(Alloc.Vec.t_Vec
+                            (Alloc.Vec.t_Vec (bool & u128) Alloc.Alloc.t_Global)
+                            Alloc.Alloc.t_Global &
+                          Alloc.Vec.t_Vec (Alloc.Vec.t_Vec u128 Alloc.Alloc.t_Global)
+                            Alloc.Alloc.t_Global) =
+                          temp_0_
+                        in
+                        let ll, phi_l:(usize & u128) = temp_1_ in
+                        let _, ki_xj:(Polytune.Data_types.t_Mac & Polytune.Data_types.t_Key) =
+                          (xshares.[ ll ] <: Polytune.Data_types.t_Share).Polytune.Data_types._1
+                            .Polytune.Data_types._0.[ j ]
+                        in
+                        match
+                          hash128 ki_xj.Polytune.Data_types._0 <: Core.Result.t_Result u128 t_Error
+                        with
+                        | Core.Result.Result_Ok hoist7 ->
+                          let ki_xj_phi:Alloc.Vec.t_Vec (Alloc.Vec.t_Vec u128 Alloc.Alloc.t_Global)
+                            Alloc.Alloc.t_Global =
+                            Rust_primitives.Hax.Monomorphized_update_at.update_at_usize ki_xj_phi
+                              j
+                              (Rust_primitives.Hax.Monomorphized_update_at.update_at_usize (ki_xj_phi.[
+                                      j ]
+                                    <:
+                                    Alloc.Vec.t_Vec u128 Alloc.Alloc.t_Global)
+                                  ll
+                                  hoist7
+                                <:
+                                Alloc.Vec.t_Vec u128 Alloc.Alloc.t_Global)
+                          in
+                          (match
+                              hash128 (ki_xj.Polytune.Data_types._0 ^. delta.Polytune.Data_types._0
+                                  <:
+                                  u128)
+                              <:
+                              Core.Result.t_Result u128 t_Error
+                            with
+                            | Core.Result.Result_Ok hoist10 ->
+                              let uij:u128 =
+                                (hoist10 ^.
+                                  ((ki_xj_phi.[ j ] <: Alloc.Vec.t_Vec u128 Alloc.Alloc.t_Global).[ ll
+                                    ]
+                                    <:
+                                    u128)
+                                  <:
+                                  u128) ^.
+                                phi_l
+                              in
+                              let ei_uij:Alloc.Vec.t_Vec
+                                (Alloc.Vec.t_Vec (bool & u128) Alloc.Alloc.t_Global)
+                                Alloc.Alloc.t_Global =
+                                Rust_primitives.Hax.Monomorphized_update_at.update_at_usize ei_uij
+                                  j
+                                  (Alloc.Vec.impl_1__push #(bool & u128)
+                                      #Alloc.Alloc.t_Global
+                                      (ei_uij.[ j ]
+                                        <:
+                                        Alloc.Vec.t_Vec (bool & u128) Alloc.Alloc.t_Global)
+                                      ((e.[ ll ] <: bool), uij <: (bool & u128))
+                                    <:
+                                    Alloc.Vec.t_Vec (bool & u128) Alloc.Alloc.t_Global)
+                              in
+                              Core.Ops.Control_flow.ControlFlow_Continue
+                              (ei_uij, ki_xj_phi
+                                <:
+                                (Alloc.Vec.t_Vec
+                                    (Alloc.Vec.t_Vec (bool & u128) Alloc.Alloc.t_Global)
+                                    Alloc.Alloc.t_Global &
+                                  Alloc.Vec.t_Vec (Alloc.Vec.t_Vec u128 Alloc.Alloc.t_Global)
+                                    Alloc.Alloc.t_Global))
+                              <:
+                              Core.Ops.Control_flow.t_ControlFlow
+                                (Core.Ops.Control_flow.t_ControlFlow
+                                    (iimpl_951670863_ &
+                                      Core.Result.t_Result
+                                        (Alloc.Vec.t_Vec Polytune.Data_types.t_Share
+                                            Alloc.Alloc.t_Global) t_Error)
+                                    (Prims.unit &
+                                      (Alloc.Vec.t_Vec
+                                          (Alloc.Vec.t_Vec (bool & u128) Alloc.Alloc.t_Global)
+                                          Alloc.Alloc.t_Global &
+                                        Alloc.Vec.t_Vec (Alloc.Vec.t_Vec u128 Alloc.Alloc.t_Global)
+                                          Alloc.Alloc.t_Global)))
+                                (Alloc.Vec.t_Vec
+                                    (Alloc.Vec.t_Vec (bool & u128) Alloc.Alloc.t_Global)
+                                    Alloc.Alloc.t_Global &
+                                  Alloc.Vec.t_Vec (Alloc.Vec.t_Vec u128 Alloc.Alloc.t_Global)
+                                    Alloc.Alloc.t_Global)
+                            | Core.Result.Result_Err err ->
+                              Core.Ops.Control_flow.ControlFlow_Break
+                              (Core.Ops.Control_flow.ControlFlow_Break
+                                (channel,
+                                  (Core.Result.Result_Err err
+                                    <:
+                                    Core.Result.t_Result
+                                      (Alloc.Vec.t_Vec Polytune.Data_types.t_Share
+                                          Alloc.Alloc.t_Global) t_Error)
+                                  <:
+                                  (iimpl_951670863_ &
+                                    Core.Result.t_Result
+                                      (Alloc.Vec.t_Vec Polytune.Data_types.t_Share
+                                          Alloc.Alloc.t_Global) t_Error))
+                                <:
+                                Core.Ops.Control_flow.t_ControlFlow
+                                  (iimpl_951670863_ &
+                                    Core.Result.t_Result
+                                      (Alloc.Vec.t_Vec Polytune.Data_types.t_Share
+                                          Alloc.Alloc.t_Global) t_Error)
+                                  (Prims.unit &
+                                    (Alloc.Vec.t_Vec
+                                        (Alloc.Vec.t_Vec (bool & u128) Alloc.Alloc.t_Global)
+                                        Alloc.Alloc.t_Global &
+                                      Alloc.Vec.t_Vec (Alloc.Vec.t_Vec u128 Alloc.Alloc.t_Global)
+                                        Alloc.Alloc.t_Global)))
+                              <:
+                              Core.Ops.Control_flow.t_ControlFlow
+                                (Core.Ops.Control_flow.t_ControlFlow
+                                    (iimpl_951670863_ &
+                                      Core.Result.t_Result
+                                        (Alloc.Vec.t_Vec Polytune.Data_types.t_Share
+                                            Alloc.Alloc.t_Global) t_Error)
+                                    (Prims.unit &
+                                      (Alloc.Vec.t_Vec
+                                          (Alloc.Vec.t_Vec (bool & u128) Alloc.Alloc.t_Global)
+                                          Alloc.Alloc.t_Global &
+                                        Alloc.Vec.t_Vec (Alloc.Vec.t_Vec u128 Alloc.Alloc.t_Global)
+                                          Alloc.Alloc.t_Global)))
+                                (Alloc.Vec.t_Vec
+                                    (Alloc.Vec.t_Vec (bool & u128) Alloc.Alloc.t_Global)
+                                    Alloc.Alloc.t_Global &
+                                  Alloc.Vec.t_Vec (Alloc.Vec.t_Vec u128 Alloc.Alloc.t_Global)
+                                    Alloc.Alloc.t_Global))
+                        | Core.Result.Result_Err err ->
+                          Core.Ops.Control_flow.ControlFlow_Break
+                          (Core.Ops.Control_flow.ControlFlow_Break
+                            (channel,
+                              (Core.Result.Result_Err err
+                                <:
+                                Core.Result.t_Result
+                                  (Alloc.Vec.t_Vec Polytune.Data_types.t_Share Alloc.Alloc.t_Global)
+                                  t_Error)
+                              <:
+                              (iimpl_951670863_ &
+                                Core.Result.t_Result
+                                  (Alloc.Vec.t_Vec Polytune.Data_types.t_Share Alloc.Alloc.t_Global)
+                                  t_Error))
+                            <:
+                            Core.Ops.Control_flow.t_ControlFlow
+                              (iimpl_951670863_ &
+                                Core.Result.t_Result
+                                  (Alloc.Vec.t_Vec Polytune.Data_types.t_Share Alloc.Alloc.t_Global)
+                                  t_Error)
+                              (Prims.unit &
+                                (Alloc.Vec.t_Vec
+                                    (Alloc.Vec.t_Vec (bool & u128) Alloc.Alloc.t_Global)
+                                    Alloc.Alloc.t_Global &
+                                  Alloc.Vec.t_Vec (Alloc.Vec.t_Vec u128 Alloc.Alloc.t_Global)
+                                    Alloc.Alloc.t_Global)))
+                          <:
+                          Core.Ops.Control_flow.t_ControlFlow
+                            (Core.Ops.Control_flow.t_ControlFlow
+                                (iimpl_951670863_ &
+                                  Core.Result.t_Result
+                                    (Alloc.Vec.t_Vec Polytune.Data_types.t_Share
+                                        Alloc.Alloc.t_Global) t_Error)
+                                (Prims.unit &
+                                  (Alloc.Vec.t_Vec
+                                      (Alloc.Vec.t_Vec (bool & u128) Alloc.Alloc.t_Global)
+                                      Alloc.Alloc.t_Global &
+                                    Alloc.Vec.t_Vec (Alloc.Vec.t_Vec u128 Alloc.Alloc.t_Global)
+                                      Alloc.Alloc.t_Global)))
+                            (Alloc.Vec.t_Vec (Alloc.Vec.t_Vec (bool & u128) Alloc.Alloc.t_Global)
+                                Alloc.Alloc.t_Global &
+                              Alloc.Vec.t_Vec (Alloc.Vec.t_Vec u128 Alloc.Alloc.t_Global)
+                                Alloc.Alloc.t_Global))
+                  <:
+                  Core.Ops.Control_flow.t_ControlFlow
+                    (iimpl_951670863_ &
+                      Core.Result.t_Result
+                        (Alloc.Vec.t_Vec Polytune.Data_types.t_Share Alloc.Alloc.t_Global) t_Error)
+                    (Alloc.Vec.t_Vec (Alloc.Vec.t_Vec (bool & u128) Alloc.Alloc.t_Global)
+                        Alloc.Alloc.t_Global &
+                      Alloc.Vec.t_Vec (Alloc.Vec.t_Vec u128 Alloc.Alloc.t_Global)
+                        Alloc.Alloc.t_Global)
+                with
+                | Core.Ops.Control_flow.ControlFlow_Break ret ->
+                  Core.Ops.Control_flow.ControlFlow_Break
+                  (Core.Ops.Control_flow.ControlFlow_Break ret
+                    <:
+                    Core.Ops.Control_flow.t_ControlFlow
+                      (iimpl_951670863_ &
+                        Core.Result.t_Result
+                          (Alloc.Vec.t_Vec Polytune.Data_types.t_Share Alloc.Alloc.t_Global) t_Error
+                      )
+                      (Prims.unit &
+                        (Alloc.Vec.t_Vec (Alloc.Vec.t_Vec (bool & u128) Alloc.Alloc.t_Global)
+                            Alloc.Alloc.t_Global &
+                          Alloc.Vec.t_Vec (Alloc.Vec.t_Vec u128 Alloc.Alloc.t_Global)
+                            Alloc.Alloc.t_Global)))
+                  <:
+                  Core.Ops.Control_flow.t_ControlFlow
+                    (Core.Ops.Control_flow.t_ControlFlow
+                        (iimpl_951670863_ &
+                          Core.Result.t_Result
+                            (Alloc.Vec.t_Vec Polytune.Data_types.t_Share Alloc.Alloc.t_Global)
+                            t_Error)
+                        (Prims.unit &
+                          (Alloc.Vec.t_Vec (Alloc.Vec.t_Vec (bool & u128) Alloc.Alloc.t_Global)
+                              Alloc.Alloc.t_Global &
+                            Alloc.Vec.t_Vec (Alloc.Vec.t_Vec u128 Alloc.Alloc.t_Global)
+                              Alloc.Alloc.t_Global)))
+                    (Alloc.Vec.t_Vec (Alloc.Vec.t_Vec (bool & u128) Alloc.Alloc.t_Global)
+                        Alloc.Alloc.t_Global &
+                      Alloc.Vec.t_Vec (Alloc.Vec.t_Vec u128 Alloc.Alloc.t_Global)
+                        Alloc.Alloc.t_Global)
+                | Core.Ops.Control_flow.ControlFlow_Continue loop_res ->
+                  Core.Ops.Control_flow.ControlFlow_Continue loop_res
+                  <:
+                  Core.Ops.Control_flow.t_ControlFlow
+                    (Core.Ops.Control_flow.t_ControlFlow
+                        (iimpl_951670863_ &
+                          Core.Result.t_Result
+                            (Alloc.Vec.t_Vec Polytune.Data_types.t_Share Alloc.Alloc.t_Global)
+                            t_Error)
+                        (Prims.unit &
+                          (Alloc.Vec.t_Vec (Alloc.Vec.t_Vec (bool & u128) Alloc.Alloc.t_Global)
+                              Alloc.Alloc.t_Global &
+                            Alloc.Vec.t_Vec (Alloc.Vec.t_Vec u128 Alloc.Alloc.t_Global)
+                              Alloc.Alloc.t_Global)))
+                    (Alloc.Vec.t_Vec (Alloc.Vec.t_Vec (bool & u128) Alloc.Alloc.t_Global)
+                        Alloc.Alloc.t_Global &
+                      Alloc.Vec.t_Vec (Alloc.Vec.t_Vec u128 Alloc.Alloc.t_Global)
+                        Alloc.Alloc.t_Global))
+          <:
+          Core.Ops.Control_flow.t_ControlFlow
+            (iimpl_951670863_ &
+              Core.Result.t_Result
+                (Alloc.Vec.t_Vec Polytune.Data_types.t_Share Alloc.Alloc.t_Global) t_Error)
+            (Alloc.Vec.t_Vec (Alloc.Vec.t_Vec (bool & u128) Alloc.Alloc.t_Global)
+                Alloc.Alloc.t_Global &
+              Alloc.Vec.t_Vec (Alloc.Vec.t_Vec u128 Alloc.Alloc.t_Global) Alloc.Alloc.t_Global)
+        with
+        | Core.Ops.Control_flow.ControlFlow_Break ret -> ret
+        | Core.Ops.Control_flow.ControlFlow_Continue (ei_uij, ki_xj_phi) ->
+          let tmp0, out:(iimpl_951670863_ &
+            Core.Result.t_Result
+              (Alloc.Vec.t_Vec (Alloc.Vec.t_Vec (bool & u128) Alloc.Alloc.t_Global)
+                  Alloc.Alloc.t_Global) t_Error) =
+            broadcast_first_send_second #bool
+              #u128
+              #iimpl_951670863_
+              channel
+              i
+              n
+              "flaand"
+              (Core.Ops.Deref.f_deref #(Alloc.Vec.t_Vec
+                      (Alloc.Vec.t_Vec (bool & u128) Alloc.Alloc.t_Global) Alloc.Alloc.t_Global)
+                  #FStar.Tactics.Typeclasses.solve
+                  ei_uij
+                <:
+                t_Slice (Alloc.Vec.t_Vec (bool & u128) Alloc.Alloc.t_Global))
+              l
+          in
+          let channel:iimpl_951670863_ = tmp0 in
+          match
+            out
+            <:
+            Core.Result.t_Result
+              (Alloc.Vec.t_Vec (Alloc.Vec.t_Vec (bool & u128) Alloc.Alloc.t_Global)
+                  Alloc.Alloc.t_Global) t_Error
+          with
+          | Core.Result.Result_Ok ei_uij_k ->
+            (match
+                Rust_primitives.Hax.Folds.fold_return (Core.Iter.Traits.Collect.f_into_iter #(Core.Iter.Adapters.Filter.t_Filter
+                          (Core.Ops.Range.t_Range usize) (usize -> bool))
+                      #FStar.Tactics.Typeclasses.solve
+                      (Core.Iter.Traits.Iterator.f_filter #(Core.Ops.Range.t_Range usize)
+                          #FStar.Tactics.Typeclasses.solve
+                          ({ Core.Ops.Range.f_start = mk_usize 0; Core.Ops.Range.f_end = n }
+                            <:
+                            Core.Ops.Range.t_Range usize)
+                          (fun j ->
+                              let j:usize = j in
+                              j <>. i <: bool)
+                        <:
+                        Core.Iter.Adapters.Filter.t_Filter (Core.Ops.Range.t_Range usize)
+                          (usize -> bool))
+                    <:
+                    Core.Iter.Adapters.Filter.t_Filter (Core.Ops.Range.t_Range usize)
+                      (usize -> bool))
+                  (ki_xj_phi, zshares
+                    <:
+                    (Alloc.Vec.t_Vec (Alloc.Vec.t_Vec u128 Alloc.Alloc.t_Global)
+                        Alloc.Alloc.t_Global &
+                      Alloc.Vec.t_Vec Polytune.Data_types.t_Share Alloc.Alloc.t_Global))
+                  (fun temp_0_ j ->
+                      let ki_xj_phi, zshares:(Alloc.Vec.t_Vec
+                          (Alloc.Vec.t_Vec u128 Alloc.Alloc.t_Global) Alloc.Alloc.t_Global &
+                        Alloc.Vec.t_Vec Polytune.Data_types.t_Share Alloc.Alloc.t_Global) =
+                        temp_0_
+                      in
+                      let j:usize = j in
+                      match
+                        Rust_primitives.Hax.Folds.fold_return (Core.Iter.Traits.Collect.f_into_iter #(
+                                Core.Iter.Adapters.Take.t_Take
+                                (Core.Iter.Adapters.Enumerate.t_Enumerate
+                                  (Core.Slice.Iter.t_Iter Polytune.Data_types.t_Share)))
+                              #FStar.Tactics.Typeclasses.solve
+                              (Core.Iter.Traits.Iterator.f_take #(Core.Iter.Adapters.Enumerate.t_Enumerate
+                                    (Core.Slice.Iter.t_Iter Polytune.Data_types.t_Share))
+                                  #FStar.Tactics.Typeclasses.solve
+                                  (Core.Iter.Traits.Iterator.f_enumerate #(Core.Slice.Iter.t_Iter
+                                        Polytune.Data_types.t_Share)
+                                      #FStar.Tactics.Typeclasses.solve
+                                      (Core.Slice.impl__iter #Polytune.Data_types.t_Share xshares
+                                        <:
+                                        Core.Slice.Iter.t_Iter Polytune.Data_types.t_Share)
+                                    <:
+                                    Core.Iter.Adapters.Enumerate.t_Enumerate
+                                    (Core.Slice.Iter.t_Iter Polytune.Data_types.t_Share))
+                                  l
+                                <:
+                                Core.Iter.Adapters.Take.t_Take
+                                (Core.Iter.Adapters.Enumerate.t_Enumerate
+                                  (Core.Slice.Iter.t_Iter Polytune.Data_types.t_Share)))
+                            <:
+                            Core.Iter.Adapters.Take.t_Take
+                            (Core.Iter.Adapters.Enumerate.t_Enumerate
+                              (Core.Slice.Iter.t_Iter Polytune.Data_types.t_Share)))
+                          (ki_xj_phi, zshares
+                            <:
+                            (Alloc.Vec.t_Vec (Alloc.Vec.t_Vec u128 Alloc.Alloc.t_Global)
+                                Alloc.Alloc.t_Global &
+                              Alloc.Vec.t_Vec Polytune.Data_types.t_Share Alloc.Alloc.t_Global))
+                          (fun temp_0_ temp_1_ ->
+                              let ki_xj_phi, zshares:(Alloc.Vec.t_Vec
+                                  (Alloc.Vec.t_Vec u128 Alloc.Alloc.t_Global) Alloc.Alloc.t_Global &
+                                Alloc.Vec.t_Vec Polytune.Data_types.t_Share Alloc.Alloc.t_Global) =
+                                temp_0_
+                              in
+                              let ll, xbit:(usize & Polytune.Data_types.t_Share) = temp_1_ in
+                              let mi_xj, _:(Polytune.Data_types.t_Mac & Polytune.Data_types.t_Key) =
+                                (xshares.[ ll ] <: Polytune.Data_types.t_Share)
+                                  .Polytune.Data_types._1
+                                  .Polytune.Data_types._0.[ j ]
+                              in
+                              match
+                                hash128 mi_xj.Polytune.Data_types._0
+                                <:
+                                Core.Result.t_Result u128 t_Error
+                              with
+                              | Core.Result.Result_Ok hoist13 ->
+                                let ki_xj_phi:Alloc.Vec.t_Vec
+                                  (Alloc.Vec.t_Vec u128 Alloc.Alloc.t_Global) Alloc.Alloc.t_Global =
+                                  Rust_primitives.Hax.Monomorphized_update_at.update_at_usize ki_xj_phi
+                                    j
+                                    (Rust_primitives.Hax.Monomorphized_update_at.update_at_usize (ki_xj_phi.[
+                                            j ]
+                                          <:
+                                          Alloc.Vec.t_Vec u128 Alloc.Alloc.t_Global)
+                                        ll
+                                        ((((ki_xj_phi.[ j ]
+                                                <:
+                                                Alloc.Vec.t_Vec u128 Alloc.Alloc.t_Global).[ ll ]
+                                              <:
+                                              u128) ^.
+                                            hoist13
+                                            <:
+                                            u128) ^.
+                                          ((cast (xbit.Polytune.Data_types._0 <: bool) <: u128) *!
+                                            ((ei_uij_k.[ j ]
+                                                <:
+                                                Alloc.Vec.t_Vec (bool & u128) Alloc.Alloc.t_Global).[
+                                                ll ]
+                                              <:
+                                              (bool & u128))
+                                              ._2
+                                            <:
+                                            u128)
+                                          <:
+                                          u128)
+                                      <:
+                                      Alloc.Vec.t_Vec u128 Alloc.Alloc.t_Global)
+                                in
+                                let mac, key:(Polytune.Data_types.t_Mac & Polytune.Data_types.t_Key)
+                                =
+                                  (rshares.[ ll ] <: Polytune.Data_types.t_Share)
+                                    .Polytune.Data_types._1
+                                    .Polytune.Data_types._0.[ j ]
+                                in
+                                if
+                                  ((ei_uij_k.[ j ]
+                                      <:
+                                      Alloc.Vec.t_Vec (bool & u128) Alloc.Alloc.t_Global).[ ll ])
+                                    ._1
+                                then
+                                  let zshares:Alloc.Vec.t_Vec Polytune.Data_types.t_Share
+                                    Alloc.Alloc.t_Global =
+                                    Rust_primitives.Hax.Monomorphized_update_at.update_at_usize zshares
+                                      ll
+                                      ({
+                                          (zshares.[ ll ] <: Polytune.Data_types.t_Share) with
+                                          Polytune.Data_types._1
+                                          =
+                                          {
+                                            (zshares.[ ll ] <: Polytune.Data_types.t_Share)
+                                              .Polytune.Data_types._1 with
+                                            Polytune.Data_types._0
+                                            =
+                                            Rust_primitives.Hax.update_at (zshares.[ ll ]
+                                                <:
+                                                Polytune.Data_types.t_Share)
+                                                .Polytune.Data_types._1
+                                                .Polytune.Data_types._0
+                                              j
+                                              (mac,
+                                                (Polytune.Data_types.Key
+                                                  (key.Polytune.Data_types._0 ^.
+                                                    delta.Polytune.Data_types._0
+                                                    <:
+                                                    u128)
+                                                  <:
+                                                  Polytune.Data_types.t_Key)
+                                                <:
+                                                (Polytune.Data_types.t_Mac &
+                                                  Polytune.Data_types.t_Key))
+                                            <:
+                                            Smallvec.t_SmallVec
+                                            (t_Array
+                                                (Polytune.Data_types.t_Mac &
+                                                  Polytune.Data_types.t_Key) (mk_usize 2))
+                                          }
+                                          <:
+                                          Polytune.Data_types.t_Auth
+                                        }
+                                        <:
+                                        Polytune.Data_types.t_Share)
+                                  in
+                                  Core.Ops.Control_flow.ControlFlow_Continue
+                                  (ki_xj_phi, zshares
+                                    <:
+                                    (Alloc.Vec.t_Vec (Alloc.Vec.t_Vec u128 Alloc.Alloc.t_Global)
+                                        Alloc.Alloc.t_Global &
+                                      Alloc.Vec.t_Vec Polytune.Data_types.t_Share
+                                        Alloc.Alloc.t_Global))
+                                  <:
+                                  Core.Ops.Control_flow.t_ControlFlow
+                                    (Core.Ops.Control_flow.t_ControlFlow
+                                        (iimpl_951670863_ &
+                                          Core.Result.t_Result
+                                            (Alloc.Vec.t_Vec Polytune.Data_types.t_Share
+                                                Alloc.Alloc.t_Global) t_Error)
+                                        (Prims.unit &
+                                          (Alloc.Vec.t_Vec
+                                              (Alloc.Vec.t_Vec u128 Alloc.Alloc.t_Global)
+                                              Alloc.Alloc.t_Global &
+                                            Alloc.Vec.t_Vec Polytune.Data_types.t_Share
+                                              Alloc.Alloc.t_Global)))
+                                    (Alloc.Vec.t_Vec (Alloc.Vec.t_Vec u128 Alloc.Alloc.t_Global)
+                                        Alloc.Alloc.t_Global &
+                                      Alloc.Vec.t_Vec Polytune.Data_types.t_Share
+                                        Alloc.Alloc.t_Global)
+                                else
+                                  let zshares:Alloc.Vec.t_Vec Polytune.Data_types.t_Share
+                                    Alloc.Alloc.t_Global =
+                                    Rust_primitives.Hax.Monomorphized_update_at.update_at_usize zshares
+                                      ll
+                                      ({
+                                          (zshares.[ ll ] <: Polytune.Data_types.t_Share) with
+                                          Polytune.Data_types._1
+                                          =
+                                          {
+                                            (zshares.[ ll ] <: Polytune.Data_types.t_Share)
+                                              .Polytune.Data_types._1 with
+                                            Polytune.Data_types._0
+                                            =
+                                            Rust_primitives.Hax.update_at (zshares.[ ll ]
+                                                <:
+                                                Polytune.Data_types.t_Share)
+                                                .Polytune.Data_types._1
+                                                .Polytune.Data_types._0
+                                              j
+                                              (mac, key
+                                                <:
+                                                (Polytune.Data_types.t_Mac &
+                                                  Polytune.Data_types.t_Key))
+                                            <:
+                                            Smallvec.t_SmallVec
+                                            (t_Array
+                                                (Polytune.Data_types.t_Mac &
+                                                  Polytune.Data_types.t_Key) (mk_usize 2))
+                                          }
+                                          <:
+                                          Polytune.Data_types.t_Auth
+                                        }
+                                        <:
+                                        Polytune.Data_types.t_Share)
+                                  in
+                                  Core.Ops.Control_flow.ControlFlow_Continue
+                                  (ki_xj_phi, zshares
+                                    <:
+                                    (Alloc.Vec.t_Vec (Alloc.Vec.t_Vec u128 Alloc.Alloc.t_Global)
+                                        Alloc.Alloc.t_Global &
+                                      Alloc.Vec.t_Vec Polytune.Data_types.t_Share
+                                        Alloc.Alloc.t_Global))
+                                  <:
+                                  Core.Ops.Control_flow.t_ControlFlow
+                                    (Core.Ops.Control_flow.t_ControlFlow
+                                        (iimpl_951670863_ &
+                                          Core.Result.t_Result
+                                            (Alloc.Vec.t_Vec Polytune.Data_types.t_Share
+                                                Alloc.Alloc.t_Global) t_Error)
+                                        (Prims.unit &
+                                          (Alloc.Vec.t_Vec
+                                              (Alloc.Vec.t_Vec u128 Alloc.Alloc.t_Global)
+                                              Alloc.Alloc.t_Global &
+                                            Alloc.Vec.t_Vec Polytune.Data_types.t_Share
+                                              Alloc.Alloc.t_Global)))
+                                    (Alloc.Vec.t_Vec (Alloc.Vec.t_Vec u128 Alloc.Alloc.t_Global)
+                                        Alloc.Alloc.t_Global &
+                                      Alloc.Vec.t_Vec Polytune.Data_types.t_Share
+                                        Alloc.Alloc.t_Global)
+                              | Core.Result.Result_Err err ->
+                                Core.Ops.Control_flow.ControlFlow_Break
+                                (Core.Ops.Control_flow.ControlFlow_Break
+                                  (channel,
+                                    (Core.Result.Result_Err err
+                                      <:
+                                      Core.Result.t_Result
+                                        (Alloc.Vec.t_Vec Polytune.Data_types.t_Share
+                                            Alloc.Alloc.t_Global) t_Error)
+                                    <:
+                                    (iimpl_951670863_ &
+                                      Core.Result.t_Result
+                                        (Alloc.Vec.t_Vec Polytune.Data_types.t_Share
+                                            Alloc.Alloc.t_Global) t_Error))
+                                  <:
+                                  Core.Ops.Control_flow.t_ControlFlow
+                                    (iimpl_951670863_ &
+                                      Core.Result.t_Result
+                                        (Alloc.Vec.t_Vec Polytune.Data_types.t_Share
+                                            Alloc.Alloc.t_Global) t_Error)
+                                    (Prims.unit &
+                                      (Alloc.Vec.t_Vec (Alloc.Vec.t_Vec u128 Alloc.Alloc.t_Global)
+                                          Alloc.Alloc.t_Global &
+                                        Alloc.Vec.t_Vec Polytune.Data_types.t_Share
+                                          Alloc.Alloc.t_Global)))
+                                <:
+                                Core.Ops.Control_flow.t_ControlFlow
+                                  (Core.Ops.Control_flow.t_ControlFlow
+                                      (iimpl_951670863_ &
+                                        Core.Result.t_Result
+                                          (Alloc.Vec.t_Vec Polytune.Data_types.t_Share
+                                              Alloc.Alloc.t_Global) t_Error)
+                                      (Prims.unit &
+                                        (Alloc.Vec.t_Vec (Alloc.Vec.t_Vec u128 Alloc.Alloc.t_Global)
+                                            Alloc.Alloc.t_Global &
+                                          Alloc.Vec.t_Vec Polytune.Data_types.t_Share
+                                            Alloc.Alloc.t_Global)))
+                                  (Alloc.Vec.t_Vec (Alloc.Vec.t_Vec u128 Alloc.Alloc.t_Global)
+                                      Alloc.Alloc.t_Global &
+                                    Alloc.Vec.t_Vec Polytune.Data_types.t_Share Alloc.Alloc.t_Global
+                                  ))
+                        <:
+                        Core.Ops.Control_flow.t_ControlFlow
+                          (iimpl_951670863_ &
+                            Core.Result.t_Result
+                              (Alloc.Vec.t_Vec Polytune.Data_types.t_Share Alloc.Alloc.t_Global)
+                              t_Error)
+                          (Alloc.Vec.t_Vec (Alloc.Vec.t_Vec u128 Alloc.Alloc.t_Global)
+                              Alloc.Alloc.t_Global &
+                            Alloc.Vec.t_Vec Polytune.Data_types.t_Share Alloc.Alloc.t_Global)
+                      with
+                      | Core.Ops.Control_flow.ControlFlow_Break ret ->
+                        Core.Ops.Control_flow.ControlFlow_Break
+                        (Core.Ops.Control_flow.ControlFlow_Break ret
+                          <:
+                          Core.Ops.Control_flow.t_ControlFlow
+                            (iimpl_951670863_ &
+                              Core.Result.t_Result
+                                (Alloc.Vec.t_Vec Polytune.Data_types.t_Share Alloc.Alloc.t_Global)
+                                t_Error)
+                            (Prims.unit &
+                              (Alloc.Vec.t_Vec (Alloc.Vec.t_Vec u128 Alloc.Alloc.t_Global)
+                                  Alloc.Alloc.t_Global &
+                                Alloc.Vec.t_Vec Polytune.Data_types.t_Share Alloc.Alloc.t_Global)))
+                        <:
+                        Core.Ops.Control_flow.t_ControlFlow
+                          (Core.Ops.Control_flow.t_ControlFlow
+                              (iimpl_951670863_ &
+                                Core.Result.t_Result
+                                  (Alloc.Vec.t_Vec Polytune.Data_types.t_Share Alloc.Alloc.t_Global)
+                                  t_Error)
+                              (Prims.unit &
+                                (Alloc.Vec.t_Vec (Alloc.Vec.t_Vec u128 Alloc.Alloc.t_Global)
+                                    Alloc.Alloc.t_Global &
+                                  Alloc.Vec.t_Vec Polytune.Data_types.t_Share Alloc.Alloc.t_Global))
+                          )
+                          (Alloc.Vec.t_Vec (Alloc.Vec.t_Vec u128 Alloc.Alloc.t_Global)
+                              Alloc.Alloc.t_Global &
+                            Alloc.Vec.t_Vec Polytune.Data_types.t_Share Alloc.Alloc.t_Global)
+                      | Core.Ops.Control_flow.ControlFlow_Continue loop_res ->
+                        Core.Ops.Control_flow.ControlFlow_Continue loop_res
+                        <:
+                        Core.Ops.Control_flow.t_ControlFlow
+                          (Core.Ops.Control_flow.t_ControlFlow
+                              (iimpl_951670863_ &
+                                Core.Result.t_Result
+                                  (Alloc.Vec.t_Vec Polytune.Data_types.t_Share Alloc.Alloc.t_Global)
+                                  t_Error)
+                              (Prims.unit &
+                                (Alloc.Vec.t_Vec (Alloc.Vec.t_Vec u128 Alloc.Alloc.t_Global)
+                                    Alloc.Alloc.t_Global &
+                                  Alloc.Vec.t_Vec Polytune.Data_types.t_Share Alloc.Alloc.t_Global))
+                          )
+                          (Alloc.Vec.t_Vec (Alloc.Vec.t_Vec u128 Alloc.Alloc.t_Global)
+                              Alloc.Alloc.t_Global &
+                            Alloc.Vec.t_Vec Polytune.Data_types.t_Share Alloc.Alloc.t_Global))
+                <:
+                Core.Ops.Control_flow.t_ControlFlow
+                  (iimpl_951670863_ &
+                    Core.Result.t_Result
+                      (Alloc.Vec.t_Vec Polytune.Data_types.t_Share Alloc.Alloc.t_Global) t_Error)
+                  (Alloc.Vec.t_Vec (Alloc.Vec.t_Vec u128 Alloc.Alloc.t_Global) Alloc.Alloc.t_Global &
+                    Alloc.Vec.t_Vec Polytune.Data_types.t_Share Alloc.Alloc.t_Global)
+              with
+              | Core.Ops.Control_flow.ControlFlow_Break ret -> ret
+              | Core.Ops.Control_flow.ControlFlow_Continue (ki_xj_phi, zshares) ->
+                let hi:Alloc.Vec.t_Vec u128 Alloc.Alloc.t_Global =
+                  Alloc.Vec.from_elem #u128 (mk_u128 0) l
+                in
+                let commhi:Alloc.Vec.t_Vec t_Commitment Alloc.Alloc.t_Global =
+                  Alloc.Vec.impl__with_capacity #t_Commitment l
+                in
+                let commhi, hi:(Alloc.Vec.t_Vec t_Commitment Alloc.Alloc.t_Global &
+                  Alloc.Vec.t_Vec u128 Alloc.Alloc.t_Global) =
+                  Rust_primitives.Hax.Folds.fold_range (mk_usize 0)
+                    l
+                    (fun temp_0_ temp_1_ ->
+                        let commhi, hi:(Alloc.Vec.t_Vec t_Commitment Alloc.Alloc.t_Global &
+                          Alloc.Vec.t_Vec u128 Alloc.Alloc.t_Global) =
+                          temp_0_
+                        in
+                        let _:usize = temp_1_ in
+                        true)
+                    (commhi, hi
+                      <:
+                      (Alloc.Vec.t_Vec t_Commitment Alloc.Alloc.t_Global &
+                        Alloc.Vec.t_Vec u128 Alloc.Alloc.t_Global))
+                    (fun temp_0_ ll ->
+                        let commhi, hi:(Alloc.Vec.t_Vec t_Commitment Alloc.Alloc.t_Global &
+                          Alloc.Vec.t_Vec u128 Alloc.Alloc.t_Global) =
+                          temp_0_
+                        in
+                        let ll:usize = ll in
+                        let hi:Alloc.Vec.t_Vec u128 Alloc.Alloc.t_Global =
+                          Core.Iter.Traits.Iterator.f_fold (Core.Iter.Traits.Collect.f_into_iter #(Core.Iter.Adapters.Filter.t_Filter
+                                    (Core.Ops.Range.t_Range usize) (usize -> bool))
+                                #FStar.Tactics.Typeclasses.solve
+                                (Core.Iter.Traits.Iterator.f_filter #(Core.Ops.Range.t_Range usize)
+                                    #FStar.Tactics.Typeclasses.solve
+                                    ({
+                                        Core.Ops.Range.f_start = mk_usize 0;
+                                        Core.Ops.Range.f_end = n
+                                      }
+                                      <:
+                                      Core.Ops.Range.t_Range usize)
+                                    (fun k ->
+                                        let k:usize = k in
+                                        k <>. i <: bool)
+                                  <:
+                                  Core.Iter.Adapters.Filter.t_Filter (Core.Ops.Range.t_Range usize)
+                                    (usize -> bool))
+                              <:
+                              Core.Iter.Adapters.Filter.t_Filter (Core.Ops.Range.t_Range usize)
+                                (usize -> bool))
+                            hi
+                            (fun hi k ->
+                                let hi:Alloc.Vec.t_Vec u128 Alloc.Alloc.t_Global = hi in
+                                let k:usize = k in
+                                let mk_zi, ki_zk:(Polytune.Data_types.t_Mac &
+                                  Polytune.Data_types.t_Key) =
+                                  (zshares.[ ll ] <: Polytune.Data_types.t_Share)
+                                    .Polytune.Data_types._1
+                                    .Polytune.Data_types._0.[ k ]
+                                in
+                                let hi:Alloc.Vec.t_Vec u128 Alloc.Alloc.t_Global =
+                                  Rust_primitives.Hax.Monomorphized_update_at.update_at_usize hi
+                                    ll
+                                    ((((hi.[ ll ] <: u128) ^. mk_zi.Polytune.Data_types._0 <: u128) ^.
+                                        ki_zk.Polytune.Data_types._0
+                                        <:
+                                        u128) ^.
+                                      ((ki_xj_phi.[ k ] <: Alloc.Vec.t_Vec u128 Alloc.Alloc.t_Global
+                                        ).[ ll ]
+                                        <:
+                                        u128)
+                                      <:
+                                      u128)
+                                in
+                                hi)
+                        in
+                        let hi:Alloc.Vec.t_Vec u128 Alloc.Alloc.t_Global =
+                          Rust_primitives.Hax.Monomorphized_update_at.update_at_usize hi
+                            ll
+                            (((hi.[ ll ] <: u128) ^.
+                                ((cast ((xshares.[ ll ] <: Polytune.Data_types.t_Share)
+                                          .Polytune.Data_types._0
+                                        <:
+                                        bool)
+                                    <:
+                                    u128) *!
+                                  (phi.[ ll ] <: u128)
+                                  <:
+                                  u128)
+                                <:
+                                u128) ^.
+                              ((cast ((zshares.[ ll ] <: Polytune.Data_types.t_Share)
+                                        .Polytune.Data_types._0
+                                      <:
+                                      bool)
+                                  <:
+                                  u128) *!
+                                delta.Polytune.Data_types._0
+                                <:
+                                u128)
+                              <:
+                              u128)
+                        in
+                        let commhi:Alloc.Vec.t_Vec t_Commitment Alloc.Alloc.t_Global =
+                          Alloc.Vec.impl_1__push #t_Commitment
+                            #Alloc.Alloc.t_Global
+                            commhi
+                            (commit (Core.Num.impl_u128__to_be_bytes (hi.[ ll ] <: u128)
+                                  <:
+                                  t_Slice u8)
+                              <:
+                              t_Commitment)
+                        in
+                        commhi, hi
+                        <:
+                        (Alloc.Vec.t_Vec t_Commitment Alloc.Alloc.t_Global &
+                          Alloc.Vec.t_Vec u128 Alloc.Alloc.t_Global))
+                in
+                let _:Prims.unit = Core.Mem.drop #(Alloc.Vec.t_Vec u128 Alloc.Alloc.t_Global) phi in
+                let _:Prims.unit =
+                  Core.Mem.drop #(Alloc.Vec.t_Vec (Alloc.Vec.t_Vec u128 Alloc.Alloc.t_Global)
+                        Alloc.Alloc.t_Global)
+                    ki_xj_phi
+                in
+                let tmp0, out:(iimpl_951670863_ &
+                  Core.Result.t_Result
+                    (Alloc.Vec.t_Vec (Alloc.Vec.t_Vec t_Commitment Alloc.Alloc.t_Global)
+                        Alloc.Alloc.t_Global) t_Error) =
+                  broadcast #t_Commitment
+                    #iimpl_951670863_
+                    channel
+                    i
+                    n
+                    "flaand comm"
+                    (Core.Ops.Deref.f_deref #(Alloc.Vec.t_Vec t_Commitment Alloc.Alloc.t_Global)
+                        #FStar.Tactics.Typeclasses.solve
+                        commhi
+                      <:
+                      t_Slice t_Commitment)
+                    l
+                in
+                let channel:iimpl_951670863_ = tmp0 in
+                match
+                  out
+                  <:
+                  Core.Result.t_Result
+                    (Alloc.Vec.t_Vec (Alloc.Vec.t_Vec t_Commitment Alloc.Alloc.t_Global)
+                        Alloc.Alloc.t_Global) t_Error
+                with
+                | Core.Result.Result_Ok commhi_k ->
+                  let tmp0, out:(iimpl_951670863_ &
+                    Core.Result.t_Result
+                      (Alloc.Vec.t_Vec (Alloc.Vec.t_Vec u128 Alloc.Alloc.t_Global)
+                          Alloc.Alloc.t_Global) t_Error) =
+                    broadcast #u128
+                      #iimpl_951670863_
+                      channel
+                      i
+                      n
+                      "flaand hash"
+                      (Core.Ops.Deref.f_deref #(Alloc.Vec.t_Vec u128 Alloc.Alloc.t_Global)
+                          #FStar.Tactics.Typeclasses.solve
+                          hi
+                        <:
+                        t_Slice u128)
+                      l
+                  in
+                  let channel:iimpl_951670863_ = tmp0 in
+                  (match
+                      out
+                      <:
+                      Core.Result.t_Result
+                        (Alloc.Vec.t_Vec (Alloc.Vec.t_Vec u128 Alloc.Alloc.t_Global)
+                            Alloc.Alloc.t_Global) t_Error
+                    with
+                    | Core.Result.Result_Ok hi_k_outer ->
+                      let xor_all_hi:Alloc.Vec.t_Vec u128 Alloc.Alloc.t_Global = hi in
+                      (match
+                          Rust_primitives.Hax.Folds.fold_return (Core.Iter.Traits.Collect.f_into_iter
+                                #(Core.Iter.Adapters.Filter.t_Filter (Core.Ops.Range.t_Range usize)
+                                    (usize -> bool))
+                                #FStar.Tactics.Typeclasses.solve
+                                (Core.Iter.Traits.Iterator.f_filter #(Core.Ops.Range.t_Range usize)
+                                    #FStar.Tactics.Typeclasses.solve
+                                    ({
+                                        Core.Ops.Range.f_start = mk_usize 0;
+                                        Core.Ops.Range.f_end = n
+                                      }
+                                      <:
+                                      Core.Ops.Range.t_Range usize)
+                                    (fun k ->
+                                        let k:usize = k in
+                                        k <>. i <: bool)
+                                  <:
+                                  Core.Iter.Adapters.Filter.t_Filter (Core.Ops.Range.t_Range usize)
+                                    (usize -> bool))
+                              <:
+                              Core.Iter.Adapters.Filter.t_Filter (Core.Ops.Range.t_Range usize)
+                                (usize -> bool))
+                            xor_all_hi
+                            (fun xor_all_hi k ->
+                                let xor_all_hi:Alloc.Vec.t_Vec u128 Alloc.Alloc.t_Global =
+                                  xor_all_hi
+                                in
+                                let k:usize = k in
+                                match
+                                  Rust_primitives.Hax.Folds.fold_range_return (mk_usize 0)
+                                    (Alloc.Vec.impl_1__len #u128 #Alloc.Alloc.t_Global xor_all_hi
+                                      <:
+                                      usize)
+                                    (fun xor_all_hi temp_1_ ->
+                                        let xor_all_hi:Alloc.Vec.t_Vec u128 Alloc.Alloc.t_Global =
+                                          xor_all_hi
+                                        in
+                                        let _:usize = temp_1_ in
+                                        true)
+                                    xor_all_hi
+                                    (fun xor_all_hi ll ->
+                                        let xor_all_hi:Alloc.Vec.t_Vec u128 Alloc.Alloc.t_Global =
+                                          xor_all_hi
+                                        in
+                                        let ll:usize = ll in
+                                        if
+                                          ~.(open_commitment ((commhi_k.[ k ]
+                                                  <:
+                                                  Alloc.Vec.t_Vec t_Commitment Alloc.Alloc.t_Global).[
+                                                  ll ]
+                                                <:
+                                                t_Commitment)
+                                              (Core.Num.impl_u128__to_be_bytes ((hi_k_outer.[ k ]
+                                                      <:
+                                                      Alloc.Vec.t_Vec u128 Alloc.Alloc.t_Global).[ ll
+                                                    ]
+                                                    <:
+                                                    u128)
+                                                <:
+                                                t_Slice u8)
+                                            <:
+                                            bool)
+                                          <:
+                                          bool
+                                        then
+                                          Core.Ops.Control_flow.ControlFlow_Break
+                                          (Core.Ops.Control_flow.ControlFlow_Break
+                                            (channel,
+                                              (Core.Result.Result_Err
+                                                (Error_CommitmentCouldNotBeOpened <: t_Error)
+                                                <:
+                                                Core.Result.t_Result
+                                                  (Alloc.Vec.t_Vec Polytune.Data_types.t_Share
+                                                      Alloc.Alloc.t_Global) t_Error)
+                                              <:
+                                              (iimpl_951670863_ &
+                                                Core.Result.t_Result
+                                                  (Alloc.Vec.t_Vec Polytune.Data_types.t_Share
+                                                      Alloc.Alloc.t_Global) t_Error))
+                                            <:
+                                            Core.Ops.Control_flow.t_ControlFlow
+                                              (iimpl_951670863_ &
+                                                Core.Result.t_Result
+                                                  (Alloc.Vec.t_Vec Polytune.Data_types.t_Share
+                                                      Alloc.Alloc.t_Global) t_Error)
+                                              (Prims.unit &
+                                                Alloc.Vec.t_Vec u128 Alloc.Alloc.t_Global))
+                                          <:
+                                          Core.Ops.Control_flow.t_ControlFlow
+                                            (Core.Ops.Control_flow.t_ControlFlow
+                                                (iimpl_951670863_ &
+                                                  Core.Result.t_Result
+                                                    (Alloc.Vec.t_Vec Polytune.Data_types.t_Share
+                                                        Alloc.Alloc.t_Global) t_Error)
+                                                (Prims.unit &
+                                                  Alloc.Vec.t_Vec u128 Alloc.Alloc.t_Global))
+                                            (Alloc.Vec.t_Vec u128 Alloc.Alloc.t_Global)
+                                        else
+                                          Core.Ops.Control_flow.ControlFlow_Continue
+                                          (Rust_primitives.Hax.Monomorphized_update_at.update_at_usize
+                                              xor_all_hi
+                                              ll
+                                              ((xor_all_hi.[ ll ] <: u128) ^.
+                                                ((hi_k_outer.[ k ]
+                                                    <:
+                                                    Alloc.Vec.t_Vec u128 Alloc.Alloc.t_Global).[ ll
+                                                  ]
+                                                  <:
+                                                  u128)
+                                                <:
+                                                u128)
+                                            <:
+                                            Alloc.Vec.t_Vec u128 Alloc.Alloc.t_Global)
+                                          <:
+                                          Core.Ops.Control_flow.t_ControlFlow
+                                            (Core.Ops.Control_flow.t_ControlFlow
+                                                (iimpl_951670863_ &
+                                                  Core.Result.t_Result
+                                                    (Alloc.Vec.t_Vec Polytune.Data_types.t_Share
+                                                        Alloc.Alloc.t_Global) t_Error)
+                                                (Prims.unit &
+                                                  Alloc.Vec.t_Vec u128 Alloc.Alloc.t_Global))
+                                            (Alloc.Vec.t_Vec u128 Alloc.Alloc.t_Global))
+                                  <:
+                                  Core.Ops.Control_flow.t_ControlFlow
+                                    (iimpl_951670863_ &
+                                      Core.Result.t_Result
+                                        (Alloc.Vec.t_Vec Polytune.Data_types.t_Share
+                                            Alloc.Alloc.t_Global) t_Error)
+                                    (Alloc.Vec.t_Vec u128 Alloc.Alloc.t_Global)
+                                with
+                                | Core.Ops.Control_flow.ControlFlow_Break ret ->
+                                  Core.Ops.Control_flow.ControlFlow_Break
+                                  (Core.Ops.Control_flow.ControlFlow_Break ret
+                                    <:
+                                    Core.Ops.Control_flow.t_ControlFlow
+                                      (iimpl_951670863_ &
+                                        Core.Result.t_Result
+                                          (Alloc.Vec.t_Vec Polytune.Data_types.t_Share
+                                              Alloc.Alloc.t_Global) t_Error)
+                                      (Prims.unit & Alloc.Vec.t_Vec u128 Alloc.Alloc.t_Global))
+                                  <:
+                                  Core.Ops.Control_flow.t_ControlFlow
+                                    (Core.Ops.Control_flow.t_ControlFlow
+                                        (iimpl_951670863_ &
+                                          Core.Result.t_Result
+                                            (Alloc.Vec.t_Vec Polytune.Data_types.t_Share
+                                                Alloc.Alloc.t_Global) t_Error)
+                                        (Prims.unit & Alloc.Vec.t_Vec u128 Alloc.Alloc.t_Global))
+                                    (Alloc.Vec.t_Vec u128 Alloc.Alloc.t_Global)
+                                | Core.Ops.Control_flow.ControlFlow_Continue loop_res ->
+                                  Core.Ops.Control_flow.ControlFlow_Continue loop_res
+                                  <:
+                                  Core.Ops.Control_flow.t_ControlFlow
+                                    (Core.Ops.Control_flow.t_ControlFlow
+                                        (iimpl_951670863_ &
+                                          Core.Result.t_Result
+                                            (Alloc.Vec.t_Vec Polytune.Data_types.t_Share
+                                                Alloc.Alloc.t_Global) t_Error)
+                                        (Prims.unit & Alloc.Vec.t_Vec u128 Alloc.Alloc.t_Global))
+                                    (Alloc.Vec.t_Vec u128 Alloc.Alloc.t_Global))
+                          <:
+                          Core.Ops.Control_flow.t_ControlFlow
+                            (iimpl_951670863_ &
+                              Core.Result.t_Result
+                                (Alloc.Vec.t_Vec Polytune.Data_types.t_Share Alloc.Alloc.t_Global)
+                                t_Error) (Alloc.Vec.t_Vec u128 Alloc.Alloc.t_Global)
+                        with
+                        | Core.Ops.Control_flow.ControlFlow_Break ret -> ret
+                        | Core.Ops.Control_flow.ControlFlow_Continue xor_all_hi ->
+                          let _, out:(Core.Iter.Adapters.Take.t_Take (Core.Slice.Iter.t_Iter u128) &
+                            bool) =
+                            Core.Iter.Traits.Iterator.f_any #(Core.Iter.Adapters.Take.t_Take
+                                (Core.Slice.Iter.t_Iter u128))
+                              #FStar.Tactics.Typeclasses.solve
+                              (Core.Iter.Traits.Iterator.f_take #(Core.Slice.Iter.t_Iter u128)
+                                  #FStar.Tactics.Typeclasses.solve
+                                  (Core.Slice.impl__iter #u128
+                                      (Core.Ops.Deref.f_deref #(Alloc.Vec.t_Vec u128
+                                              Alloc.Alloc.t_Global)
+                                          #FStar.Tactics.Typeclasses.solve
+                                          xor_all_hi
+                                        <:
+                                        t_Slice u128)
+                                    <:
+                                    Core.Slice.Iter.t_Iter u128)
+                                  l
+                                <:
+                                Core.Iter.Adapters.Take.t_Take (Core.Slice.Iter.t_Iter u128))
+                              (fun xh ->
+                                  let xh:u128 = xh in
+                                  xh <>. mk_u128 0 <: bool)
+                          in
+                          if out
+                          then
+                            channel,
+                            (Core.Result.Result_Err (Error_LaANDXorNotZero <: t_Error)
+                              <:
+                              Core.Result.t_Result
+                                (Alloc.Vec.t_Vec Polytune.Data_types.t_Share Alloc.Alloc.t_Global)
+                                t_Error)
+                            <:
+                            (iimpl_951670863_ &
+                              Core.Result.t_Result
+                                (Alloc.Vec.t_Vec Polytune.Data_types.t_Share Alloc.Alloc.t_Global)
+                                t_Error)
+                          else
+                            let hax_temp_output:Core.Result.t_Result
+                              (Alloc.Vec.t_Vec Polytune.Data_types.t_Share Alloc.Alloc.t_Global)
+                              t_Error =
+                              Core.Result.Result_Ok zshares
+                              <:
+                              Core.Result.t_Result
+                                (Alloc.Vec.t_Vec Polytune.Data_types.t_Share Alloc.Alloc.t_Global)
+                                t_Error
+                            in
+                            channel, hax_temp_output
+                            <:
+                            (iimpl_951670863_ &
+                              Core.Result.t_Result
+                                (Alloc.Vec.t_Vec Polytune.Data_types.t_Share Alloc.Alloc.t_Global)
+                                t_Error))
+                    | Core.Result.Result_Err err ->
+                      channel,
+                      (Core.Result.Result_Err err
+                        <:
+                        Core.Result.t_Result
+                          (Alloc.Vec.t_Vec Polytune.Data_types.t_Share Alloc.Alloc.t_Global) t_Error
+                      )
+                      <:
+                      (iimpl_951670863_ &
+                        Core.Result.t_Result
+                          (Alloc.Vec.t_Vec Polytune.Data_types.t_Share Alloc.Alloc.t_Global) t_Error
+                      ))
+                | Core.Result.Result_Err err ->
+                  channel,
+                  (Core.Result.Result_Err err
+                    <:
+                    Core.Result.t_Result
+                      (Alloc.Vec.t_Vec Polytune.Data_types.t_Share Alloc.Alloc.t_Global) t_Error)
+                  <:
+                  (iimpl_951670863_ &
+                    Core.Result.t_Result
+                      (Alloc.Vec.t_Vec Polytune.Data_types.t_Share Alloc.Alloc.t_Global) t_Error))
+          | Core.Result.Result_Err err ->
+            channel,
+            (Core.Result.Result_Err err
+              <:
+              Core.Result.t_Result
+                (Alloc.Vec.t_Vec Polytune.Data_types.t_Share Alloc.Alloc.t_Global) t_Error)
+            <:
+            (iimpl_951670863_ &
+              Core.Result.t_Result
+                (Alloc.Vec.t_Vec Polytune.Data_types.t_Share Alloc.Alloc.t_Global) t_Error))
+    | Core.Result.Result_Err err ->
+      channel,
+      (Core.Result.Result_Err err
+        <:
+        Core.Result.t_Result (Alloc.Vec.t_Vec Polytune.Data_types.t_Share Alloc.Alloc.t_Global)
+          t_Error)
+      <:
+      (iimpl_951670863_ &
+        Core.Result.t_Result (Alloc.Vec.t_Vec Polytune.Data_types.t_Share Alloc.Alloc.t_Global)
+          t_Error)
